src/program_proof/simplepb/pb_setstate_proof.v
@@ -1,0 +1,177 @@
+From Perennial.program_proof Require Import grove_prelude.
+From Goose.github_com.mit_pdos.gokv.simplepb Require Export pb.
+From Perennial.program_proof.grove_shared Require Import urpc_proof urpc_spec.
+From Perennial.program_proof.simplepb Require Export pb_ghost.
+From Perennial.program_proof.simplepb Require Import pb_marshal_proof.
+From Perennial.program_proof Require Import marshal_stateless_proof.
+From Perennial.program_proof.simplepb Require Import pb_definitions.
+
+Section pb_setstate_proof.
+Context `{!heapGS Σ, !stagedG Σ}.
+Context {pb_record:PBRecord}.
+
+Notation OpType := (pb_OpType pb_record).
+Notation has_op_encoding := (pb_has_op_encoding pb_record).
+Notation has_snap_encoding := (pb_has_snap_encoding pb_record).
+Notation has_op_encoding_injective := (pb_has_op_encoding_injective pb_record).
+Notation compute_reply := (pb_compute_reply pb_record).
+Notation pbG := (pbG (pb_record:=pb_record)).
+
+Context `{!waitgroupG Σ}.
+Context `{!pbG Σ}.
+
+Lemma wp_Clerk__SetState γ γsrv ck args_ptr (epoch:u64) σ snap :
+  {{{
+        "#Hck" ∷ is_Clerk ck γ γsrv ∗
+        "#Hprop_lb" ∷ is_proposal_lb γ epoch σ ∗
+        "#Hprop_facts" ∷ is_proposal_facts γ epoch σ ∗
+        "%Henc" ∷ ⌜has_snap_encoding snap (fst <$> σ)⌝ ∗
+        "%Hno_overflow" ∷ ⌜length σ = int.nat (length σ)⌝ ∗
+        "Hargs" ∷ SetStateArgs.own args_ptr (SetStateArgs.mkC epoch (length σ) snap)
+  }}}
+    Clerk__SetState #ck #args_ptr
+  {{{
+        (err:u64), RET #err;
+        □(if (decide (err = U64 0)) then
+            is_epoch_lb γsrv epoch ∗
+            is_accepted_lb γsrv epoch σ
+          else
+            True)
+  }}}.
+Proof.
+  iIntros (Φ) "Hpre HΦ".
+  iNamed "Hpre".
+  wp_call.
+  wp_apply (wp_ref_of_zero).
+  { done. }
+  iIntros (rep) "Hrep".
+  wp_pures.
+  iNamed "Hck".
+  wp_apply (SetStateArgs.wp_Encode with "[$Hargs]").
+  iIntros (enc_args enc_args_sl) "(%Henc_args & Henc_args_sl & Hargs)".
+  wp_loadField.
+  iDestruct (is_slice_to_small with "Henc_args_sl") as "Henc_args_sl".
+  wp_apply (wp_frame_wand with "HΦ").
+  wp_apply (wp_Client__Call2 with "Hcl_rpc [] Henc_args_sl Hrep").
+  {
+    iDestruct "Hsrv" as "[_ [$ _]]".
+  }
+  { (* Successful RPC *)
+    iModIntro.
+    iNext.
+    unfold SetState_spec.
+    iExists _, _.
+    iSplitR; first done.
+    iSplitR; first done.
+    simpl.
+    iSplitR.
+    { iPureIntro. done. }
+    iFrame "Hprop_lb Hprop_facts".
+    iSplit.
+    { (* No error from RPC, state was accepted *)
+      iIntros "#Hepoch_lb #Hacc".
+      iIntros (?) "%Henc_rep Hargs_sl".
+      iIntros (?) "Hrep Hrep_sl".
+      wp_pures.
+      wp_load.
+
+      (* FIXME: separate lemma *)
+      wp_call.
+      rewrite Henc_rep.
+      wp_apply (wp_ReadInt with "Hrep_sl").
+      iIntros (?) "_".
+      wp_pures.
+      iModIntro.
+      iIntros "HΦ".
+      iApply "HΦ".
+      iFrame "Hacc Hepoch_lb".
+    }
+    { (* SetState was rejected by the server (e.g. stale epoch number) *)
+      iIntros (err) "%Herr_nz".
+      iIntros.
+      wp_pures.
+      wp_load.
+      wp_call.
+      rewrite H.
+      wp_apply (wp_ReadInt with "[$]").
+      iIntros.
+      wp_pures.
+      iModIntro.
+      iIntros "HΦ".
+      iApply "HΦ".
+      iFrame.
+      iModIntro.
+      destruct (decide _).
+      {
+        exfalso. done.
+      }
+      {
+        done.
+      }
+    }
+  }
+  { (* RPC error *)
+    iIntros.
+    wp_pures.
+    wp_if_destruct.
+    {
+      iModIntro.
+      iIntros "HΦ".
+      iApply "HΦ".
+      destruct (decide (_)).
+      { exfalso. done. }
+      { done. }
+    }
+    { exfalso. done. }
+  }
+Qed.
+
+Lemma wp_Server__SetState γ γsrv s args_ptr args σ Φ :
+  is_Server s γ γsrv -∗
+  SetStateArgs.own args_ptr args -∗
+  SetState_core_spec γ γsrv args σ (λ err, Φ #err) -∗
+  WP pb.Server__SetState #s #args_ptr {{ Φ }}
+  .
+Proof.
+  iIntros "#His_srv Hargs HΦ".
+  iNamed "His_srv".
+  wp_call.
+  wp_loadField.
+  wp_apply (acquire_spec with "[$HmuInv]").
+  iIntros "[Hlocked Hown]".
+  wp_pures.
+  iNamed "Hown".
+  iNamed "Hargs".
+  wp_loadField.
+  wp_loadField.
+  wp_if_destruct.
+  { (* stale epoch *)
+    wp_loadField.
+    unfold SetState_core_spec.
+    iDestruct "HΦ" as "(_ & _ & _ & _ & HΦ)".
+    iRight in "HΦ".
+    wp_apply (release_spec with "[-HΦ]").
+    {
+      iFrame "HmuInv Hlocked".
+      iNext.
+      iExists _, _, _, _, _, _, _.
+      iFrame "∗#%".
+    }
+    wp_pures.
+    iApply "HΦ".
+    done.
+  }
+  { (* successfully set the state *)
+    wp_loadField.
+    wp_loadField.
+    wp_if_destruct.
+    { (* state has been set previously. Use is_prop_lb to get agreement. *)
+      wp_loadField.
+
+      admit.
+    }
+    admit.
+  }
+Admitted.
+
+End pb_setstate_proof.
